\noindent\textbf{Basic}

\begin{equation*}
C_n = C_{2n}^{n} - C_{2n}^{n - 1} = \frac{1}{n + 1} C^{n}_{2n}
\end{equation*}

\begin{equation*}
C_n = \frac{1}{n+1} \sum_{i=0}^{n} (C_n^i)^2
\end{equation*}

\begin{equation*}
C_{n+1} = \frac{2(2n+1)}{n+2}C_n, \quad C_0 = 1
\end{equation*}

\begin{equation*}
C_{n+1} = \sum_{i=0}^{n} C_iC_{n-i}, \quad C_0 = 1
\end{equation*}

\noindent\textbf{DP and Extra}

We construct a sequence only contains $-1$ and $1$. It satisfys the maximal prefix sum is less than or equal to $0$, i.e.

\begin{equation*}
\max_j\left\{{\sum_{i=1}^{j}a_i}\right\} \leq 0
\end{equation*}

We define $f(x,y)$ is using the number of $-1$ is $x$, and the number of $1$ is $y$. Then

\begin{equation*}
\begin{aligned}
f(x,y) &= f(x-1,y) + f(x,y-1) &\quad (x >= y) \\
f(x,y) &= 0 &\quad (x < y) \\
f(x,y) &= 1 &\quad (x > 0, y = 0)
\end{aligned}
\end{equation*}

It can be regarded as appending a new $1$ to the ending or a new $-1$, and they cannot increase the maximal prefix sum because of the condition $x >= y$. After appending, the new prefix sum is $y - x$, which is less than or equal to $0$.

In addtion, $f(x, y) = C_{x+y}^x - C_{x+y}^{x+1} \quad (x \geq y)$

