\noindent\textbf{Property}

\begin{equation*}
C_n^k=\frac{k}{n} C_{n-1}^{k-1}
\end{equation*}

\begin{equation*}
C_n^m=C_{n-1}^m + C_{n-1}^{m-1}
\end{equation*}

\begin{equation*}
\sum_{i=0}^{n} C_n^i = 2^n
\end{equation*}

\begin{equation*}
\sum_{i=0}^{n} (-1)^i C_n^i = 0
\end{equation*}

\begin{equation*}
C_{m+n}^m=\sum_{i=0}^{m}C_n^iC_{m}^{m-i}=\sum_{i=0}^{m}C_{n}^iC_m^i \quad (n \ge m)
\end{equation*}

\begin{equation*}
\sum_{i=0}^n (C_n^i)^2 = C_{2n}^n
\end{equation*}

\begin{equation*}
\sum_{i=0}^n iC_n^i = n2^{n-1}
\end{equation*}

\begin{equation*}
\sum_{i=0}^n i^2C_n^i = n(n+1)2^{n-2}
\end{equation*}

\begin{equation*}
\sum_{l=0}^{r}C_l^k = C_{n+1}^{k+1}
\end{equation*}

\begin{equation*}
C_n^rC_r^k = C_n^kC_{n-k}^{r-k}
\end{equation*}

\begin{equation*}
\sum_{i=0}^{n} C_{n-i}^i = Fib(n+1)
\end{equation*}

